New integer parsers based on FStar.Endianness and LowStar.Endianness

src/lowparse/LowParse.Low.BoundedInt.fst
@@ -7,7 +7,8 @@ module U32 = FStar.UInt32
 module HST = FStar.HyperStack.ST
 module HS = FStar.HyperStack
 module B = LowStar.Buffer
-module E = LowParse.BigEndianImpl.Low
+module E = LowParse.Endianness
+module LE = LowParse.Low.Endianness
 module Cast = FStar.Int.Cast
 
 friend LowParse.Spec.BoundedInt
@@ -15,14 +16,16 @@ friend LowParse.Spec.BoundedInt
 (* bounded integers *)
 
 let read_bounded_integer_1 () =
-  [@inline_let] let _ =
+  [@inline_let]
+  let _ =
     decode_bounded_integer_injective 1
   in
   make_total_constant_size_reader 1 1ul #(bounded_integer 1) (decode_bounded_integer 1) () (fun #rrel #rel input pos ->
     let h = HST.get () in
-    let r = E.be_to_n_1 _ _ (E.u32 ()) input pos in
+    E.index_be_to_n (Seq.slice (B.as_seq h input) (U32.v pos) (U32.v pos + 1)) 0;
     E.lemma_be_to_n_is_bounded (Seq.slice (B.as_seq h input) (U32.v pos) (U32.v pos + 1));
-    r
+    let r = B.index input pos in
+    Cast.uint8_to_uint32 r
   )
 
 let read_bounded_integer_2 () =
@@ -31,12 +34,10 @@ let read_bounded_integer_2 () =
   in
   make_total_constant_size_reader 2 2ul #(bounded_integer 2) (decode_bounded_integer 2) () (fun #rrel #rel input pos ->
     let h = HST.get () in
-    let r = E.be_to_n_2 _ _ (E.u32 ()) input pos in
+    let r = LE.load16_be_i (* #(Ghost.hide rrel) #(Ghost.hide rel) *) input pos in
     E.lemma_be_to_n_is_bounded (Seq.slice (B.as_seq h input) (U32.v pos) (U32.v pos + 2));
-    r
+    Cast.uint16_to_uint32 r
   )
-
-#push-options "--z3rlimit 16"
 
 let read_bounded_integer_3 () =
   [@inline_let] let _ =
@@ -44,9 +45,14 @@ let read_bounded_integer_3 () =
   in
   make_total_constant_size_reader 3 3ul #(bounded_integer 3) (decode_bounded_integer 3) () (fun #rrel #rel input pos ->
     let h = HST.get () in
-    let r = E.be_to_n_3 _ _ (E.u32 ()) input pos in
+    Seq.lemma_split (Seq.slice (B.as_seq h input) (U32.v pos) (U32.v pos + 3)) 2;
+    E.reveal_be_to_n (Seq.slice (B.as_seq h input) (U32.v pos) (U32.v pos + 3));
+    let lo = B.index input (pos `U32.add` 2ul) in
+    let hi = LE.load16_be_i (* #(Ghost.hide rrel) #(Ghost.hide rel) *) input pos in
+    E.lemma_be_to_n_is_bounded (Seq.slice (B.as_seq h input) (U32.v pos) (U32.v pos + 2));
     E.lemma_be_to_n_is_bounded (Seq.slice (B.as_seq h input) (U32.v pos) (U32.v pos + 3));
-    r
+    assert_norm (pow2 8 == 256);
+    Cast.uint8_to_uint32 lo `U32.add` (256ul `U32.mul` Cast.uint16_to_uint32 hi)
   )
 
 let read_bounded_integer_4 () =
@@ -55,33 +61,60 @@ let read_bounded_integer_4 () =
   in
   make_total_constant_size_reader 4 4ul #(bounded_integer 4) (decode_bounded_integer 4) () (fun #rrel #rel input pos ->
     let h = HST.get () in
-    let r = E.be_to_n_4 _ _ (E.u32 ()) input pos in
     E.lemma_be_to_n_is_bounded (Seq.slice (B.as_seq h input) (U32.v pos) (U32.v pos + 4));
-    r
+    LE.load32_be_i (* #(Ghost.hide rrel) #(Ghost.hide rel) *) input pos
   )
-
-#pop-options
 
 let serialize32_bounded_integer_1 () =
   fun (v: bounded_integer 1) #rrel #rel out pos ->
-  E.n_to_be_1 _ _ (E.u32 ()) v out pos;
+  bounded_integer_prop_equiv 1 v;
+  E.index_n_to_be 1 (U32.v v) 0;
+  mbuffer_upd out (Ghost.hide (U32.v pos)) (Ghost.hide (U32.v pos + 1)) pos (Cast.uint32_to_uint8 v);
   1ul
 
 let serialize32_bounded_integer_2 () =
   fun (v: bounded_integer 2) #rrel #rel out pos ->
-  E.n_to_be_2 _ _ (E.u32 ()) v out pos;
+  bounded_integer_prop_equiv 2 v;
+  let h = HST.get () in
+  let v' = (Cast.uint32_to_uint16 v) in
+  LE.writable_store_pre out (U32.v pos) 2 (fun s -> E.be_to_n s == U16.v v') h;
+  LE.store16_be_i (* #(Ghost.hide rrel) #(Ghost.hide rel) *) out pos v';
+  let h' = HST.get () in
+  LE.store_post_modifies out (U32.v pos) 2 (fun s -> E.be_to_n s == U16.v v') h h';
   2ul
 
-#push-options "--z3rlimit 50"
+#push-options "--z3rlimit 16"
+
 let serialize32_bounded_integer_3 () =
   fun (v: bounded_integer 3) #rrel #rel out pos ->
-  E.n_to_be_3 _ _ (E.u32 ()) v out pos;
+  bounded_integer_prop_equiv 3 v;
+  E.reveal_n_to_be 3 (U32.v v);
+  assert_norm (pow2 8 == 256);
+  let lo = Cast.uint32_to_uint8 v in
+  mbuffer_upd out (Ghost.hide (U32.v pos)) (Ghost.hide (U32.v pos + 3)) (pos `U32.add` 2ul) lo;
+  let hi' = v `U32.div` 256ul in
+  FStar.Math.Lemmas.small_mod (U32.v hi') (pow2 16);
+  let hi = Cast.uint32_to_uint16 hi' in
+  let h1 = HST.get () in
+  LE.writable_weaken out (U32.v pos) (U32.v pos + 3) h1 (U32.v pos) (U32.v pos + 2);
+  LE.writable_store_pre out (U32.v pos) 2 (fun s -> E.be_to_n s == U16.v hi) h1;
+  LE.store16_be_i (* #(Ghost.hide rrel) #(Ghost.hide rel) *) out pos hi;
+  let h2 = HST.get () in
+  LE.store_post_modifies out (U32.v pos) 2 (fun s -> E.be_to_n s == U16.v hi) h1 h2;
+  B.modifies_buffer_from_to_elim out (pos `U32.add` 2ul) (pos `U32.add` 3ul) (B.loc_buffer_from_to out pos (pos `U32.add` 2ul)) h1 h2;
+  assert (Seq.slice (B.as_seq h2 out) (U32.v pos + 2) (U32.v pos + 3) `Seq.equal` Seq.create 1 lo);
   3ul
+
 #pop-options
 
 let serialize32_bounded_integer_4 () =
   fun (v: bounded_integer 4) #rrel #rel out pos ->
-  E.n_to_be_4 _ _ (E.u32 ()) v out pos;
+  bounded_integer_prop_equiv 4 v;
+  let h = HST.get () in
+  LE.writable_store_pre out (U32.v pos) 4 (fun s -> E.be_to_n s == U32.v v) h;
+  LE.store32_be_i (* #(Ghost.hide rrel) #(Ghost.hide rel) *) out pos v;
+  let h' = HST.get () in
+  LE.store_post_modifies out (U32.v pos) 4 (fun s -> E.be_to_n s == U32.v v) h h';
   4ul
 
 inline_for_extraction
@@ -231,7 +264,8 @@ let read_bounded_integer_le_1 =
   [@inline_let] let _ = bounded_integer_of_le_injective 1 in
   make_total_constant_size_reader 1 1ul #(bounded_integer 1) (bounded_integer_of_le 1) () (fun #rrel #rel b pos ->
     let h = HST.get () in
-    [@inline_let] let _ = bounded_integer_of_le_1_eq (Seq.slice (B.as_seq h b) (U32.v pos) (U32.v pos + 1)) in
+    E.index_le_to_n (Seq.slice (B.as_seq h b) (U32.v pos) (U32.v pos + 1)) 0;
+    E.lemma_le_to_n_is_bounded (Seq.slice (B.as_seq h b) (U32.v pos) (U32.v pos + 1));
     let r = B.index b pos in
     Cast.uint8_to_uint32 r
   )
@@ -240,37 +274,32 @@ let read_bounded_integer_le_2 =
   [@inline_let] let _ = bounded_integer_of_le_injective 2 in
   make_total_constant_size_reader 2 2ul #(bounded_integer 2) (bounded_integer_of_le 2) () (fun #rrel #rel b pos ->
     let h = HST.get () in
-    [@inline_let] let _ = bounded_integer_of_le_2_eq (Seq.slice (B.as_seq h b) (U32.v pos) (U32.v pos + 2)) in
-    let r0 = B.index b pos in
-    let r1 = B.index b (pos `U32.add` 1ul) in
-    Cast.uint8_to_uint32 r0 `U32.add` (256ul `U32.mul` Cast.uint8_to_uint32 r1)
+    let r = LE.load16_le_i (* #(Ghost.hide rrel) #(Ghost.hide rel) *) b pos in
+    E.lemma_le_to_n_is_bounded (Seq.slice (B.as_seq h b) (U32.v pos) (U32.v pos + 2));
+    Cast.uint16_to_uint32 r
   )
-
-#push-options "--z3rlimit 40"
 
 let read_bounded_integer_le_3 =
   [@inline_let] let _ = bounded_integer_of_le_injective 3 in
   make_total_constant_size_reader 3 3ul #(bounded_integer 3) (bounded_integer_of_le 3) () (fun #rrel #rel b pos ->
     let h = HST.get () in
-    [@inline_let] let _ = bounded_integer_of_le_3_eq (Seq.slice (B.as_seq h b) (U32.v pos) (U32.v pos + 3)) in
-    let r0 = B.index b pos in
-    let r1 = B.index b (pos `U32.add` 1ul) in
-    let r2 = B.index b (pos `U32.add` 2ul) in
-    Cast.uint8_to_uint32 r0 `U32.add` (256ul `U32.mul` (Cast.uint8_to_uint32 r1 `U32.add` (256ul `U32.mul` Cast.uint8_to_uint32 r2)))
+    Seq.lemma_split (Seq.slice (B.as_seq h b) (U32.v pos) (U32.v pos + 3)) 1;
+    E.reveal_le_to_n (Seq.slice (B.as_seq h b) (U32.v pos) (U32.v pos + 3));
+    let lo = B.index b pos in
+    let hi = LE.load16_le_i (* #(Ghost.hide rrel) #(Ghost.hide rel) *) b (pos `U32.add` 1ul) in
+    E.lemma_le_to_n_is_bounded (Seq.slice (B.as_seq h b) (U32.v pos + 1) (U32.v pos + 3));
+    E.lemma_le_to_n_is_bounded (Seq.slice (B.as_seq h b) (U32.v pos) (U32.v pos + 3));
+    assert_norm (pow2 8 == 256);
+    Cast.uint8_to_uint32 lo `U32.add` (256ul `U32.mul` Cast.uint16_to_uint32 hi)
   )
 
 let read_bounded_integer_le_4 =
   [@inline_let] let _ = bounded_integer_of_le_injective 4 in
   make_total_constant_size_reader 4 4ul #(bounded_integer 4) (bounded_integer_of_le 4) () (fun #rrel #rel b pos ->
     let h = HST.get () in
-    [@inline_let] let _ = bounded_integer_of_le_4_eq (Seq.slice (B.as_seq h b) (U32.v pos) (U32.v pos + 4)) in
-    let r0 = B.index b pos in
-    let r1 = B.index b (pos `U32.add` 1ul) in
-    let r2 = B.index b (pos `U32.add` 2ul) in
-    let r3 = B.index b (pos `U32.add` 3ul) in
-    Cast.uint8_to_uint32 r0 `U32.add` (256ul `U32.mul` (Cast.uint8_to_uint32 r1 `U32.add` (256ul `U32.mul` (Cast.uint8_to_uint32 r2 `U32.add` (256ul `U32.mul` Cast.uint8_to_uint32 r3)))))
+    E.lemma_le_to_n_is_bounded (Seq.slice (B.as_seq h b) (U32.v pos) (U32.v pos + 4));
+    LE.load32_le_i (* #(Ghost.hide rrel) #(Ghost.hide rel) *) b pos
   )
-#pop-options
 
 let read_u16_le =
   [@inline_let] let _ = synth_u16_le_injective in
@@ -289,76 +318,58 @@ let read_u32_le =
 
 let serialize32_bounded_integer_le_1
 = fun x #rrel #rel b pos ->
-  [@inline_let]
-  let _ = serialize_bounded_integer_le_1_eq x 0 in
-  let r0 = (Cast.uint32_to_uint8 x <: U8.t) in
-  mbuffer_upd b (Ghost.hide (U32.v pos)) (Ghost.hide (U32.v pos + 1)) pos r0;
+  bounded_integer_prop_equiv 1 x;
+  E.index_n_to_le 1 (U32.v x) 0;
+  mbuffer_upd b (Ghost.hide (U32.v pos)) (Ghost.hide (U32.v pos + 1)) pos (Cast.uint32_to_uint8 x);
   1ul
 
 let write_bounded_integer_le_1
 = leaf_writer_strong_of_serializer32 serialize32_bounded_integer_le_1 ()
 
-#push-options "--z3rlimit 16"
-
 let serialize32_bounded_integer_le_2
 = fun x #rrel #rel b pos ->
-  [@inline_let]
-  let _ =
-    serialize_bounded_integer_le_2_eq x 0;
-    serialize_bounded_integer_le_2_eq x 1
-  in
-  let r0 = (Cast.uint32_to_uint8 x <: U8.t) in
-  let d0 = x `U32.div` 256ul in
-  let r1 = (Cast.uint32_to_uint8 d0 <: U8.t) in
-  mbuffer_upd b (Ghost.hide (U32.v pos)) (Ghost.hide (U32.v pos + 2)) pos r0;
-  mbuffer_upd b (Ghost.hide (U32.v pos)) (Ghost.hide (U32.v pos + 2)) (pos `U32.add` 1ul) r1;
+  bounded_integer_prop_equiv 2 x;
+  let h = HST.get () in
+  let x' = (Cast.uint32_to_uint16 x) in
+  LE.writable_store_pre b (U32.v pos) 2 (fun s -> E.le_to_n s == U16.v x') h;
+  LE.store16_le_i (* #(Ghost.hide rrel) #(Ghost.hide rel) *) b pos x';
+  let h' = HST.get () in
+  LE.store_post_modifies b (U32.v pos) 2 (fun s -> E.le_to_n s == U16.v x') h h';
   2ul
 
 let write_bounded_integer_le_2 = leaf_writer_strong_of_serializer32 serialize32_bounded_integer_le_2 ()
 
 let serialize32_bounded_integer_le_3
-= fun x #rrel #rel b pos ->
-  [@inline_let]
-  let _ =
-    serialize_bounded_integer_le_3_eq x 0;
-    serialize_bounded_integer_le_3_eq x 1;
-    serialize_bounded_integer_le_3_eq x 2
-  in
-  let r0 = (Cast.uint32_to_uint8 x <: U8.t) in
-  let d0 = x `U32.div` 256ul in
-  let r1 = (Cast.uint32_to_uint8 d0 <: U8.t) in
-  let d1 = d0 `U32.div` 256ul in
-  let r2 = (Cast.uint32_to_uint8 d1<: U8.t) in
-  mbuffer_upd b (Ghost.hide (U32.v pos)) (Ghost.hide (U32.v pos + 3)) pos r0;
-  mbuffer_upd b (Ghost.hide (U32.v pos)) (Ghost.hide (U32.v pos + 3)) (pos `U32.add` 1ul) r1;
-  mbuffer_upd b (Ghost.hide (U32.v pos)) (Ghost.hide (U32.v pos + 3)) (pos `U32.add` 2ul) r2;
+= fun v #rrel #rel out pos ->
+  bounded_integer_prop_equiv 3 v;
+  E.reveal_n_to_le 3 (U32.v v);
+  assert_norm (pow2 8 == 256);
+  let lo = Cast.uint32_to_uint8 v in
+  mbuffer_upd out (Ghost.hide (U32.v pos)) (Ghost.hide (U32.v pos + 3)) pos lo;
+  let hi' = v `U32.div` 256ul in
+  FStar.Math.Lemmas.small_mod (U32.v hi') (pow2 16);
+  let hi = Cast.uint32_to_uint16 hi' in
+  let h1 = HST.get () in
+  LE.writable_weaken out (U32.v pos) (U32.v pos + 3) h1 (U32.v pos + 1) (U32.v pos + 3);
+  LE.writable_store_pre out (U32.v pos + 1) 2 (fun s -> E.le_to_n s == U16.v hi) h1;
+  LE.store16_le_i (* #(Ghost.hide rrel) #(Ghost.hide rel) *) out (pos `U32.add` 1ul) hi;
+  let h2 = HST.get () in
+  LE.store_post_modifies out (U32.v pos + 1) 2 (fun s -> E.le_to_n s == U16.v hi) h1 h2;
+  B.modifies_buffer_from_to_elim out pos (pos `U32.add` 1ul) (B.loc_buffer_from_to out (pos `U32.add` 1ul) (pos `U32.add` 3ul)) h1 h2;
+  assert (Seq.slice (B.as_seq h2 out) (U32.v pos) (U32.v pos + 1) `Seq.equal` Seq.create 1 lo);
   3ul
 
 let write_bounded_integer_le_3 = leaf_writer_strong_of_serializer32 serialize32_bounded_integer_le_3 ()
 
 let serialize32_bounded_integer_le_4
-= fun x #rrel #rel b pos ->
-  [@inline_let]
-  let _ =
-    serialize_bounded_integer_le_4_eq x 0;
-    serialize_bounded_integer_le_4_eq x 1;
-    serialize_bounded_integer_le_4_eq x 2;
-    serialize_bounded_integer_le_4_eq x 3
-  in
-  let r0 = (Cast.uint32_to_uint8 x <: U8.t) in
-  let d0 = x `U32.div` 256ul in
-  let r1 = (Cast.uint32_to_uint8 d0 <: U8.t) in
-  let d1 = d0 `U32.div` 256ul in
-  let r2 = (Cast.uint32_to_uint8 d1<: U8.t) in
-  let d2 = d1 `U32.div` 256ul in
-  let r3 = (Cast.uint32_to_uint8 d2<: U8.t) in
-  mbuffer_upd b (Ghost.hide (U32.v pos)) (Ghost.hide (U32.v pos + 4)) pos r0;
-  mbuffer_upd b (Ghost.hide (U32.v pos)) (Ghost.hide (U32.v pos + 4)) (pos `U32.add` 1ul) r1;
-  mbuffer_upd b (Ghost.hide (U32.v pos)) (Ghost.hide (U32.v pos + 4)) (pos `U32.add` 2ul) r2;
-  mbuffer_upd b (Ghost.hide (U32.v pos)) (Ghost.hide (U32.v pos + 4)) (pos `U32.add` 3ul) r3;
+= fun v #rrel #rel out pos ->
+  bounded_integer_prop_equiv 4 v;
+  let h = HST.get () in
+  LE.writable_store_pre out (U32.v pos) 4 (fun s -> E.le_to_n s == U32.v v) h;
+  LE.store32_le_i (* #(Ghost.hide rrel) #(Ghost.hide rel) *) out pos v;
+  let h' = HST.get () in
+  LE.store_post_modifies out (U32.v pos) 4 (fun s -> E.le_to_n s == U32.v v) h h';
   4ul
-
-#pop-options
 
 let write_bounded_integer_le_4 = leaf_writer_strong_of_serializer32 serialize32_bounded_integer_le_4 ()
 
