src/lowparse/LowParse.Spec.BoundedInt.fst
@@ -3,7 +3,7 @@ module LowParse.Spec.BoundedInt
 open LowParse.Spec.Combinators // for make_total_constant_size_parser_precond
 
 module Seq = FStar.Seq
-module E = LowParse.BigEndian
+module E = FStar.Endianness
 module U8  = FStar.UInt8
 module U16 = FStar.UInt16
 module U32 = FStar.UInt32
@@ -13,6 +13,17 @@ module Cast = FStar.Int.Cast
 (* bounded integers *)
 
 let integer_size_values i = ()
+
+let bounded_integer_prop_equiv
+  (i: integer_size)
+  (u: U32.t)
+: Lemma
+  (bounded_integer_prop i u <==> U32.v u < pow2 (8 * i))
+= 
+  assert_norm (pow2 8 == 256);
+  assert_norm (pow2 16 == 65536);
+  assert_norm (pow2 24 == 16777216);
+  assert_norm (pow2 32 == 4294967296)
 
 #push-options "--z3rlimit 16"
 
@@ -52,17 +63,21 @@ let parse_bounded_integer
 = decode_bounded_integer_injective i;
   make_total_constant_size_parser i (bounded_integer i) (decode_bounded_integer i)
 
-#push-options "--max_ifuel 1 --initial_ifuel 1 --max_fuel 5 --initial_fuel 5 --z3rlimit 32"
-
-let parse_bounded_integer_spec i input = ()
-
-#pop-options
+let parse_bounded_integer_spec i input =
+  parser_kind_prop_equiv (parse_bounded_integer_kind i) (parse_bounded_integer i);
+  M.pow2_le_compat 32 (8 `FStar.Mul.op_Star` i);
+  match parse (parse_bounded_integer i) input with
+  | None -> ()
+  | Some (y, consumed) ->
+    let input' = Seq.slice input 0 i in
+    E.lemma_be_to_n_is_bounded input';
+    parse_strong_prefix (parse_bounded_integer i) input input'
 
 let serialize_bounded_integer'
   (sz: integer_size)
 : Tot (bare_serializer (bounded_integer sz))
 = (fun (x: bounded_integer sz) ->
-    let res = E.n_to_be (U32.uint_to_t sz) (U32.v x) in
+    let res = E.n_to_be sz (U32.v x) in
     res
   )
 
@@ -88,10 +103,7 @@ sz
 = serialize_bounded_integer_correct sz;
   serialize_bounded_integer' sz
 
-#push-options "--max_ifuel 4 --z3rlimit 50"
-
 let serialize_bounded_integer_spec sz x = ()
-
 
 let bounded_integer_of_le
   (i: integer_size)
@@ -136,11 +148,7 @@ let synth_u16_le
 : Tot U16.t
 = Cast.uint32_to_uint16 x
 
-#push-options "--z3rlimit 32"
-
 let synth_u16_le_injective : squash (synth_injective synth_u16_le) = ()
-
-#pop-options
 
 let parse_u16_le = parse_bounded_integer_le 2 `parse_synth` synth_u16_le
 
@@ -156,9 +164,10 @@ let serialize_bounded_integer_le'
   (sz: integer_size)
 : Tot (bare_serializer (bounded_integer sz))
 = (fun (x: bounded_integer sz) ->
-    let res = E.n_to_le (U32.uint_to_t sz) (U32.v x) in
-    res
+    E.n_to_le sz (U32.v x)
   )
+
+#push-options "--z3rlimit 16"
 
 let serialize_bounded_integer_le_correct
   (sz: integer_size)
@@ -176,6 +185,8 @@ let serialize_bounded_integer_le_correct
   in
   Classical.forall_intro prf
 
+#pop-options
+
 let serialize_bounded_integer_le
 sz
 = serialize_bounded_integer_le_correct sz;
@@ -187,11 +198,7 @@ let synth_u16_le_recip
 : Tot (bounded_integer 2)
 = Cast.uint16_to_uint32 x
 
-#push-options "--z3rlimit 32"
-
 let synth_u16_le_inverse : squash (synth_inverse synth_u16_le synth_u16_le_recip) = ()
-
-#pop-options
 
 let serialize_u16_le : serializer parse_u16_le =
   serialize_synth
@@ -214,115 +221,6 @@ let serialize_u32_le =
     (serialize_bounded_integer_le 4)
     synth_u32_le_recip
     ()
-
-#pop-options
-
-#push-options "--max_fuel 5 --z3rlimit 16"
-
-let bounded_integer_of_le_1_eq
-  (b: bytes { Seq.length b == 1 } )
-: Lemma
-  (U32.v (bounded_integer_of_le 1 b) == U8.v (Seq.index b 0))
-= assert_norm (pow2 8 == 256);
-  E.lemma_le_to_n_is_bounded b;
-  M.pow2_le_compat 32 (8 `FStar.Mul.op_Star` 1)
-
-let bounded_integer_of_le_2_eq
-  (b: bytes { Seq.length b == 2 } )
-: Lemma
-  (U32.v (bounded_integer_of_le 2 b) == U8.v (Seq.index b 0) + 256 `FStar.Mul.op_Star` U8.v (Seq.index b 1))
-= assert_norm (pow2 8 == 256);
-  E.lemma_le_to_n_is_bounded b;
-  M.pow2_le_compat 32 (8 `FStar.Mul.op_Star` 2)
-
-let bounded_integer_of_le_3_eq
-  (b: bytes { Seq.length b == 3 } )
-: Lemma
-  (U32.v (bounded_integer_of_le 3 b) == U8.v (Seq.index b 0) + 256 `FStar.Mul.op_Star` (U8.v (Seq.index b 1) + 256 `FStar.Mul.op_Star` U8.v (Seq.index b 2)))
-= assert_norm (pow2 8 == 256);
-  E.lemma_le_to_n_is_bounded b;
-  M.pow2_le_compat 32 (8 `FStar.Mul.op_Star` 3)
-
-let bounded_integer_of_le_4_eq
-  (b: bytes { Seq.length b == 4 } )
-: Lemma
-  (U32.v (bounded_integer_of_le 4 b) == U8.v (Seq.index b 0) + 256 `FStar.Mul.op_Star` (U8.v (Seq.index b 1) + 256 `FStar.Mul.op_Star` (U8.v (Seq.index b 2) + 256 `FStar.Mul.op_Star` U8.v (Seq.index b 3))))
-= assert_norm (pow2 8 == 256);
-  E.lemma_le_to_n_is_bounded b;
-  M.pow2_le_compat 32 (8 `FStar.Mul.op_Star` 4)
-
-#pop-options
-
-#push-options "--max_fuel 5 --z3rlimit 64"
-
-let serialize_bounded_integer_le_1_eq
-  (x: bounded_integer 1)
-  (i: nat { i < 1 } )
-: Lemma
-  (U8.v (Seq.index (serialize (serialize_bounded_integer_le 1) x) i) == U32.v x % 256)
-= assert_norm (pow2 8 == 256)
-
-let serialize_bounded_integer_le_2_eq
-  (x: bounded_integer 2)
-  (i: nat { i < 2 } )
-: Lemma
-  (U8.v (Seq.index (serialize (serialize_bounded_integer_le 2) x) i) == (
-    let rem = U32.v x % 256 in
-    let div = U32.v x / 256 in
-    if i = 0
-    then rem
-    else div % 256
-  ))
-= assert_norm (pow2 8 == 256)
-
-#pop-options
-
-#push-options "--z3rlimit 64"
-#restart-solver
-
-let serialize_bounded_integer_le_3_eq
-  (x: bounded_integer 3)
-  (i: nat { i < 3 } )
-: Lemma
-  (U8.v (Seq.index (serialize (serialize_bounded_integer_le 3) x) i) == (
-    let rem0 = U32.v x % 256 in
-    let div0 = U32.v x / 256 in
-    let rem1 = div0 % 256 in
-    let div1 = div0 / 256 in
-    if i = 0
-    then rem0
-    else if i = 1
-    then rem1
-    else div1 % 256
-  ))
-= assert_norm (pow2 8 == 256)
-
-#pop-options
-
-#push-options "--max_fuel 6 --z3rlimit 64"
-
-let serialize_bounded_integer_le_4_eq
-  (x: bounded_integer 4)
-  (i: nat { i < 4 } )
-: Lemma
-  (U8.v (Seq.index (serialize (serialize_bounded_integer_le 4) x) i) == (
-    let rem0 = U32.v x % 256 in
-    let div0 = U32.v x / 256 in
-    let rem1 = div0 % 256 in
-    let div1 = div0 / 256 in
-    let rem2 = div1 % 256 in
-    let div2 = div1 / 256 in
-    if i = 0
-    then rem0
-    else if i = 1
-    then rem1
-    else if i = 2
-    then rem2
-    else div2 % 256
-  ))
-= assert_norm (pow2 8 == 256)
-
-#pop-options
 
 let parse_bounded_int32
   min max
