src/lowparse/LowParse.Spec.Int.fst
@@ -1,37 +1,177 @@
 module LowParse.Spec.Int
+open LowParse.Spec.Combinators
 
-module Aux = LowParse.Spec.Int.Aux
+let decode_u8
+  (b: bytes { Seq.length b == 1 } )
+: GTot U8.t
+= Seq.index b 0
 
-let parse_u8 = Aux.parse_u8
+let decode_u8_injective () : Lemma
+  (make_total_constant_size_parser_precond 1 U8.t decode_u8)
+= ()
 
-let parse_u8_spec b = Aux.parse_u8_spec b
+let parse_u8 =
+  decode_u8_injective ();
+  make_total_constant_size_parser 1 U8.t decode_u8
+
+let parse_u8_spec
+  b
+=
+  Seq.lemma_index_slice b 0 1 0;
+  E.reveal_be_to_n (Seq.slice b 0 1);
+  E.reveal_be_to_n (Seq.slice (Seq.slice b 0 1) 0 0)
 
 let parse_u8_spec' b = ()
 
-let serialize_u8 = Aux.serialize_u8
+let serialize_u8 =
+  Seq.create 1
 
 let serialize_u8_spec x = ()
 
-let parse_u16 = Aux.parse_u16
+let decode_u16
+  (b: bytes { Seq.length b == 2 } )
+: GTot U16.t
+= E.lemma_be_to_n_is_bounded b;
+  U16.uint_to_t (E.be_to_n b)
 
-let parse_u16_spec b = Aux.parse_u16_spec b
+let decode_u16_injective'
+  (b1: bytes { Seq.length b1 == 2 } )
+  (b2: bytes { Seq.length b2 == 2 } )
+: Lemma
+  (decode_u16 b1 == decode_u16 b2 ==> Seq.equal b1 b2)
+= if decode_u16 b1 = decode_u16 b2
+  then begin
+    E.lemma_be_to_n_is_bounded b1;
+    E.lemma_be_to_n_is_bounded b2;
+    assert (U32.v (U32.uint_to_t (E.be_to_n b1)) == E.be_to_n b1);
+    assert (U32.v (U32.uint_to_t (E.be_to_n b2)) == E.be_to_n b2);
+    assert (E.be_to_n b1 == E.be_to_n b2);
+    E.be_to_n_inj b1 b2
+  end else ()
 
-let serialize_u16 = Aux.serialize_u16
+let decode_u16_injective
+  ()
+: Lemma
+  (make_total_constant_size_parser_precond 2 U16.t decode_u16)
+= Classical.forall_intro_2 decode_u16_injective'
 
-let parse_u32 = Aux.parse_u32
+let parse_u16 =
+  decode_u16_injective ();
+  make_total_constant_size_parser 2 U16.t decode_u16
 
-let parse_u32_spec = Aux.parse_u32_spec
+let parse_u16_spec
+  b
+=
+  E.lemma_be_to_n_is_bounded (Seq.slice b 0 2)
 
-let serialize_u32 = Aux.serialize_u32
+let serialize_u16 =
+  (fun (x: U16.t) -> E.n_to_be 2 (U16.v x))
 
-let parse_u64 = Aux.parse_u64
+let decode_u32
+  (b: bytes { Seq.length b == 4 } )
+: GTot U32.t
+= E.lemma_be_to_n_is_bounded b;
+  U32.uint_to_t (E.be_to_n b)
 
-let parse_u64_spec = Aux.parse_u64_spec
+let decode_u32_injective'
+  (b1: bytes { Seq.length b1 == 4 } )
+  (b2: bytes { Seq.length b2 == 4 } )
+: Lemma
+  (decode_u32 b1 == decode_u32 b2 ==> Seq.equal b1 b2)
+= if decode_u32 b1 = decode_u32 b2
+  then begin
+    E.lemma_be_to_n_is_bounded b1;
+    E.lemma_be_to_n_is_bounded b2;
+    assert (U32.v (U32.uint_to_t (E.be_to_n b1)) == E.be_to_n b1);
+    assert (U32.v (U32.uint_to_t (E.be_to_n b2)) == E.be_to_n b2);
+    assert (E.be_to_n b1 == E.be_to_n b2);
+    E.be_to_n_inj b1 b2
+  end else ()
 
-let serialize_u64 = Aux.serialize_u64
+let decode_u32_injective () : Lemma
+  (make_total_constant_size_parser_precond 4 U32.t decode_u32)
+= Classical.forall_intro_2 decode_u32_injective'
 
-let parse_u64_le = Aux.parse_u64_le
+let parse_u32 =
+  decode_u32_injective ();
+  make_total_constant_size_parser 4 U32.t decode_u32
 
-let parse_u64_le_spec = Aux.parse_u64_le_spec
+let parse_u32_spec
+  b
+=
+  E.lemma_be_to_n_is_bounded (Seq.slice b 0 4)
 
-let serialize_u64_le = Aux.serialize_u64_le
+let serialize_u32 =
+  (fun (x: U32.t) -> E.n_to_be 4 (U32.v x))
+
+let decode_u64
+  (b: bytes { Seq.length b == 8 } )
+: GTot U64.t
+= E.lemma_be_to_n_is_bounded b;
+  U64.uint_to_t (E.be_to_n b)
+
+let decode_u64_injective'
+  (b1: bytes { Seq.length b1 == 8 } )
+  (b2: bytes { Seq.length b2 == 8 } )
+: Lemma
+  (decode_u64 b1 == decode_u64 b2 ==> Seq.equal b1 b2)
+= if decode_u64 b1 = decode_u64 b2
+  then begin
+    E.lemma_be_to_n_is_bounded b1;
+    E.lemma_be_to_n_is_bounded b2;
+    assert (U64.v (U64.uint_to_t (E.be_to_n b1)) == E.be_to_n b1);
+    assert (U64.v (U64.uint_to_t (E.be_to_n b2)) == E.be_to_n b2);
+    assert (E.be_to_n b1 == E.be_to_n b2);
+    E.be_to_n_inj b1 b2
+  end else ()
+
+let decode_u64_injective () : Lemma
+  (make_total_constant_size_parser_precond 8 U64.t decode_u64)
+= Classical.forall_intro_2 decode_u64_injective'
+
+let parse_u64 =
+  decode_u64_injective ();
+  make_total_constant_size_parser 8 U64.t decode_u64
+
+let parse_u64_spec
+  b
+= E.lemma_be_to_n_is_bounded (Seq.slice b 0 8)
+
+let serialize_u64 =
+  (fun (x: U64.t) -> E.n_to_be 8 (U64.v x))
+
+let decode_u64_le
+  (b: bytes { Seq.length b == 8 } )
+: GTot U64.t
+= E.lemma_le_to_n_is_bounded b;
+  U64.uint_to_t (E.le_to_n b)
+
+let decode_u64_le_injective'
+  (b1: bytes { Seq.length b1 == 8 } )
+  (b2: bytes { Seq.length b2 == 8 } )
+: Lemma
+  (decode_u64_le b1 == decode_u64_le b2 ==> Seq.equal b1 b2)
+= if decode_u64_le b1 = decode_u64_le b2
+  then begin
+    E.lemma_le_to_n_is_bounded b1;
+    E.lemma_le_to_n_is_bounded b2;
+    assert (U64.v (U64.uint_to_t (E.le_to_n b1)) == E.le_to_n b1);
+    assert (U64.v (U64.uint_to_t (E.le_to_n b2)) == E.le_to_n b2);
+    assert (E.le_to_n b1 == E.le_to_n b2);
+    E.le_to_n_inj b1 b2
+  end else ()
+
+let decode_u64_le_injective () : Lemma
+  (make_total_constant_size_parser_precond 8 U64.t decode_u64_le)
+= Classical.forall_intro_2 decode_u64_le_injective'
+
+let parse_u64_le =
+  decode_u64_le_injective ();
+  make_total_constant_size_parser 8 U64.t decode_u64_le
+
+let parse_u64_le_spec
+  b
+= E.lemma_le_to_n_is_bounded (Seq.slice b 0 8)
+
+let serialize_u64_le =
+  (fun (x: U64.t) -> E.n_to_le 8 (U64.v x))
