src/lowparse/LowParse.Low.Int.fst
@@ -1,60 +1,106 @@
 module LowParse.Low.Int
 open LowParse.Low.Combinators
 
-module Aux = LowParse.Low.Int.Aux
-module Unique = LowParse.Spec.Int.Unique
 module Seq = FStar.Seq
 module U8  = FStar.UInt8
 module U16 = FStar.UInt16
 module U32 = FStar.UInt32
+module U64 = FStar.UInt64
 module HST = FStar.HyperStack.ST
 module HS = FStar.HyperStack
 module B = LowStar.Buffer
+module E = FStar.Endianness
+module LE = LowParse.Low.Endianness
 
-inline_for_extraction
-let read_u8 =
-  leaf_reader_ext Aux.read_u8 parse_u8 (fun x -> Unique.parse_u8_unique x)
+friend LowParse.Spec.Int
+
+let read_u8 : leaf_reader parse_u8 =
+  decode_u8_injective ();
+  make_total_constant_size_reader 1 1ul
+    decode_u8
+    ()
+    (fun #rrel #rel b pos -> B.index b pos)
 
 inline_for_extraction
 let read_u16 =
-  leaf_reader_ext Aux.read_u16 parse_u16 (fun x -> Unique.parse_u16_unique x)
+  decode_u16_injective ();
+  make_total_constant_size_reader 2 2ul
+    #U16.t
+    decode_u16
+    ()
+    (fun #rrel #rel sl pos ->
+      LE.load16_be_i (* #(Ghost.hide rrel) #(Ghost.hide rel) *) sl pos)
 
 inline_for_extraction
 let read_u32 =
-  leaf_reader_ext Aux.read_u32 parse_u32 (fun x -> Unique.parse_u32_unique x)
+  decode_u32_injective ();
+  make_total_constant_size_reader 4 4ul
+    #U32.t
+    decode_u32
+    ()
+    (fun #rrel #rel sl pos ->
+      LE.load32_be_i (* #(Ghost.hide rrel) #(Ghost.hide rel) *) sl pos)
 
 inline_for_extraction
 let read_u64 =
-  leaf_reader_ext Aux.read_u64 parse_u64 (fun x -> Unique.parse_u64_unique x)
+  decode_u64_injective ();
+  make_total_constant_size_reader 8 8ul
+    #U64.t
+    decode_u64
+    ()
+    (fun #rrel #rel sl pos ->
+      LE.load64_be_i (* #(Ghost.hide rrel) #(Ghost.hide rel) *) sl pos)
 
 inline_for_extraction
 let read_u64_le =
-  leaf_reader_ext Aux.read_u64_le parse_u64_le (fun x -> Unique.parse_u64_le_unique x)
+  decode_u64_le_injective ();
+  make_total_constant_size_reader 8 8ul
+    #U64.t
+    decode_u64_le
+    ()
+    (fun #rrel #rel sl pos ->
+      LE.load64_le_i (* #(Ghost.hide rrel) #(Ghost.hide rel) *) sl pos)
 
 inline_for_extraction
 let serialize32_u8 : serializer32 serialize_u8 = fun v #rrel #rel b pos ->
-  [@inline_let] let _ = Unique.serialize_u8_unique v in
-  Aux.serialize32_u8 v b pos
+  mbuffer_upd b (Ghost.hide (U32.v pos)) (Ghost.hide (U32.v pos + 1)) pos v;
+  1ul
 
 inline_for_extraction
 let serialize32_u16 : serializer32 serialize_u16 = fun v #rrel #rel b pos ->
-  [@inline_let] let _ = Unique.serialize_u16_unique v in
-  Aux.serialize32_u16 v b pos
+  let h = HST.get () in
+  LE.writable_store_pre b (U32.v pos) 2 (fun s -> E.be_to_n s == U16.v v) h;
+  LE.store16_be_i (* #(Ghost.hide rrel) #(Ghost.hide rel) *) b pos v;
+  let h' = HST.get () in
+  LE.store_post_modifies b (U32.v pos) 2 (fun s -> E.be_to_n s == U16.v v) h h';
+  2ul
 
 inline_for_extraction
 let serialize32_u32 : serializer32 serialize_u32 = fun v #rrel #rel b pos ->
-  [@inline_let] let _ = Unique.serialize_u32_unique v in
-  Aux.serialize32_u32 v b pos
+  let h = HST.get () in
+  LE.writable_store_pre b (U32.v pos) 4 (fun s -> E.be_to_n s == U32.v v) h;
+  LE.store32_be_i (* #(Ghost.hide rrel) #(Ghost.hide rel) *) b pos v;
+  let h' = HST.get () in
+  LE.store_post_modifies b (U32.v pos) 4 (fun s -> E.be_to_n s == U32.v v) h h';
+  4ul
 
 inline_for_extraction
 let serialize32_u64 : serializer32 serialize_u64 = fun v #rrel #rel b pos ->
-  [@inline_let] let _ = Unique.serialize_u64_unique v in
-  Aux.serialize32_u64 v b pos
+  let h = HST.get () in
+  LE.writable_store_pre b (U32.v pos) 8 (fun s -> E.be_to_n s == U64.v v) h;
+  LE.store64_be_i (* #(Ghost.hide rrel) #(Ghost.hide rel) *) b pos v;
+  let h' = HST.get () in
+  LE.store_post_modifies b (U32.v pos) 8 (fun s -> E.be_to_n s == U64.v v) h h';
+  8ul
 
 inline_for_extraction
 let serialize32_u64_le : serializer32 serialize_u64_le = fun v #rrel #rel b pos ->
-  [@inline_let] let _ = Unique.serialize_u64_le_unique v in
-  Aux.serialize32_u64_le v b pos
+  let h = HST.get () in
+  LE.writable_store_pre b (U32.v pos) 8 (fun s -> E.le_to_n s == U64.v v) h;
+  LE.store64_le_i (* #(Ghost.hide rrel) #(Ghost.hide rel) *) b pos v;
+  let h' = HST.get () in
+  LE.store_post_modifies b (U32.v pos) 8 (fun s -> E.le_to_n s == U64.v v) h h';
+  8ul
 
 let write_u8 = leaf_writer_strong_of_serializer32 serialize32_u8 ()
 
