src/lowparse/LowParse.SLow.BoundedInt.fst
@@ -7,43 +7,51 @@ module U8  = FStar.UInt8
 module U16 = FStar.UInt16
 module U32 = FStar.UInt32
 module B32 = FStar.Bytes
-module E = LowParse.BigEndianImpl.SLow
+module E = LowParse.SLow.Endianness
+module EI = LowParse.Spec.Endianness.Instances
 module Cast = FStar.Int.Cast
 
 friend LowParse.Spec.BoundedInt
 
+inline_for_extraction
+noextract
+let be_to_n_1 = norm [delta_attr [`%E.must_reduce]; iota; zeta; primops] (E.mk_be_to_n (EI.bounded_integer 1) 1)
 
 inline_for_extraction
 let decode32_bounded_integer_1
   (b: B32.lbytes 1)
 : Tot (y: bounded_integer 1 { y == decode_bounded_integer 1 (B32.reveal b) } )
-= let r = E.be_to_n_1 _ _ (E.u32 ()) b in
-  E.lemma_be_to_n_is_bounded (B32.reveal b);
-  (r <: (r: bounded_integer 1 { r == decode_bounded_integer 1 (B32.reveal b) } ))
+= be_to_n_1 b
+
+inline_for_extraction
+noextract
+let be_to_n_2 = norm [delta_attr [`%E.must_reduce]; iota; zeta; primops] (E.mk_be_to_n (EI.bounded_integer 2) 2)
 
 inline_for_extraction
 let decode32_bounded_integer_2
   (b: B32.lbytes 2)
 : Tot (y: bounded_integer 2 { y == decode_bounded_integer 2 (B32.reveal b) } )
-= let r = E.be_to_n_2 _ _ (E.u32 ()) b in
-  E.lemma_be_to_n_is_bounded (B32.reveal b);
-  (r <: (r: bounded_integer 2 { r == decode_bounded_integer 2 (B32.reveal b) } ))
+= be_to_n_2 b
+
+inline_for_extraction
+noextract
+let be_to_n_3 = norm [delta_attr [`%E.must_reduce]; iota; zeta; primops] (E.mk_be_to_n (EI.bounded_integer 3) 3)
 
 inline_for_extraction
 let decode32_bounded_integer_3
   (b: B32.lbytes 3)
 : Tot (y: bounded_integer 3 { y == decode_bounded_integer 3 (B32.reveal b) } )
-= let r = E.be_to_n_3 _ _ (E.u32 ()) b in
-  E.lemma_be_to_n_is_bounded (B32.reveal b);
-  (r <: (r: bounded_integer 3 { r == decode_bounded_integer 3 (B32.reveal b) } ))
+= be_to_n_3 b
+
+inline_for_extraction
+noextract
+let be_to_n_4 = norm [delta_attr [`%E.must_reduce]; iota; zeta; primops] (E.mk_be_to_n (EI.bounded_integer 4) 4)
 
 inline_for_extraction
 let decode32_bounded_integer_4
   (b: B32.lbytes 4)
 : Tot (y: bounded_integer 4 { y == decode_bounded_integer 4 (B32.reveal b) } )
-= let r = E.be_to_n_4 _ _ (E.u32 ()) b in
-  E.lemma_be_to_n_is_bounded (B32.reveal b);
-  (r <: (r: bounded_integer 4 { r == decode_bounded_integer 4 (B32.reveal b) } ))
+= be_to_n_4 b
 
 inline_for_extraction
 let decode32_bounded_integer
@@ -72,117 +80,110 @@ let parse32_bounded_integer_3 = parse32_bounded_integer' 3
 let parse32_bounded_integer_4 = parse32_bounded_integer' 4
 
 inline_for_extraction
+noextract
+let n_to_be_1 = norm [delta_attr [`%E.must_reduce]; iota; zeta; primops] (E.mk_n_to_be (EI.bounded_integer 1) 1)
+
+inline_for_extraction
 let serialize32_bounded_integer_1
 : (serializer32 (serialize_bounded_integer 1))
 = (fun (input: bounded_integer 1) ->
-    let b = E.n_to_be_1 _ _ (E.u32 ()) input in
-    (b <: (res: B32.bytes { serializer32_correct (serialize_bounded_integer 1) input res } ))
-  )
+    n_to_be_1 input)
+
+inline_for_extraction
+noextract
+let n_to_be_2 = norm [delta_attr [`%E.must_reduce]; iota; zeta; primops] (E.mk_n_to_be (EI.bounded_integer 2) 2)
 
 inline_for_extraction
 let serialize32_bounded_integer_2
 : (serializer32 (serialize_bounded_integer 2))
 = (fun (input: bounded_integer 2) ->
-    let b = E.n_to_be_2 _ _ (E.u32 ()) input in
-    (b <: (res: B32.bytes { serializer32_correct (serialize_bounded_integer 2) input res } ))
-  )
+    n_to_be_2 input)
+
+inline_for_extraction
+noextract
+let n_to_be_3 = norm [delta_attr [`%E.must_reduce]; iota; zeta; primops] (E.mk_n_to_be (EI.bounded_integer 3) 3)
 
 inline_for_extraction
 let serialize32_bounded_integer_3
 : (serializer32 (serialize_bounded_integer 3))
 = (fun (input: bounded_integer 3) ->
-    let b = E.n_to_be_3 _ _ (E.u32 ()) input in
-    (b <: (res: B32.bytes { serializer32_correct (serialize_bounded_integer 3) input res } ))
-  )
+    n_to_be_3 input)
+
+inline_for_extraction
+noextract
+let n_to_be_4 = norm [delta_attr [`%E.must_reduce]; iota; zeta; primops] (E.mk_n_to_be (EI.bounded_integer 4) 4)
 
 inline_for_extraction
 let serialize32_bounded_integer_4
 : (serializer32 (serialize_bounded_integer 4))
 = (fun (input: bounded_integer 4) ->
-    let b = E.n_to_be_4 _ _ (E.u32 ()) input in
-    (b <: (res: B32.bytes { serializer32_correct (serialize_bounded_integer 4) input res } ))
-  )
+    n_to_be_4 input)
+
+inline_for_extraction
+noextract
+let le_to_n_1 = norm [delta_attr [`%E.must_reduce]; iota; zeta; primops] (E.mk_le_to_n (EI.bounded_integer 1) 1)
 
 inline_for_extraction
 let bounded_integer_of_le_32_1
   (b: B32.lbytes 1)
 : Tot (y: bounded_integer 1 { y == bounded_integer_of_le 1 (B32.reveal b) } )
-= [@inline_let] let _ =
-    bounded_integer_of_le_1_eq (B32.reveal b)
-  in
-  Cast.uint8_to_uint32 (B32.get b 0ul)
+= le_to_n_1 b
+
+inline_for_extraction
+noextract
+let le_to_n_2 = norm [delta_attr [`%E.must_reduce]; iota; zeta; primops] (E.mk_le_to_n (EI.bounded_integer 2) 2)
 
 inline_for_extraction
 let bounded_integer_of_le_32_2
   (b: B32.lbytes 2)
 : Tot (y: bounded_integer 2 { y == bounded_integer_of_le 2 (B32.reveal b) } )
-= [@inline_let] let _ =
-    bounded_integer_of_le_2_eq (B32.reveal b)
-  in
-  Cast.uint8_to_uint32 (B32.get b 0ul) `U32.add` (256ul `U32.mul` Cast.uint8_to_uint32 (B32.get b 1ul))
+= le_to_n_2 b
+
+inline_for_extraction
+noextract
+let le_to_n_3 = norm [delta_attr [`%E.must_reduce]; iota; zeta; primops] (E.mk_le_to_n (EI.bounded_integer 3) 3)
 
 inline_for_extraction
 let bounded_integer_of_le_32_3
   (b: B32.lbytes 3)
 : Tot (y: bounded_integer 3 { y == bounded_integer_of_le 3 (B32.reveal b) } )
-= [@inline_let] let _ =
-    bounded_integer_of_le_3_eq (B32.reveal b)
-  in
-  Cast.uint8_to_uint32 (B32.get b 0ul) `U32.add` (256ul `U32.mul` ( Cast.uint8_to_uint32 (B32.get b 1ul) `U32.add` (256ul `U32.mul` Cast.uint8_to_uint32 (B32.get b 2ul))))
+= le_to_n_3 b
+
+inline_for_extraction
+noextract
+let le_to_n_4 = norm [delta_attr [`%E.must_reduce]; iota; zeta; primops] (E.mk_le_to_n (EI.bounded_integer 4) 4)
 
 inline_for_extraction
 let bounded_integer_of_le_32_4
   (b: B32.lbytes 4)
 : Tot (y: bounded_integer 4 { y == bounded_integer_of_le 4 (B32.reveal b) } )
-= [@inline_let] let _ =
-    bounded_integer_of_le_4_eq (B32.reveal b)
-  in
-  Cast.uint8_to_uint32 (B32.get b 0ul) `U32.add` (256ul `U32.mul` ( Cast.uint8_to_uint32 (B32.get b 1ul) `U32.add` (256ul `U32.mul` (Cast.uint8_to_uint32 (B32.get b 2ul) `U32.add` (256ul `U32.mul` Cast.uint8_to_uint32 (B32.get b 3ul))))))
+= le_to_n_4 b
 
-let parse32_bounded_integer_le_1
-= [@inline_let] let _ =
-    bounded_integer_of_le_injective 1
-  in
-  make_total_constant_size_parser32
-    1
-    1ul
-    (bounded_integer_of_le 1)
+inline_for_extraction
+let bounded_integer_of_le_32
+  (sz: integer_size)
+: Tot ((b: B32.lbytes sz) ->
+    Tot (y: bounded_integer sz { y == bounded_integer_of_le sz (B32.reveal b) } )
+  )
+= match sz with
+  | 1 -> bounded_integer_of_le_32_1
+  | 2 -> bounded_integer_of_le_32_2
+  | 3 -> bounded_integer_of_le_32_3
+  | 4 -> bounded_integer_of_le_32_4
+
+inline_for_extraction
+let parse32_bounded_integer_le' (sz: integer_size) : Tot (parser32 (parse_bounded_integer_le sz)) =
+  [@inline_let]
+  let _ = bounded_integer_of_le_injective sz in
+  make_total_constant_size_parser32 sz (U32.uint_to_t sz)
+    (bounded_integer_of_le sz)
     ()
-    bounded_integer_of_le_32_1
+    (bounded_integer_of_le_32 sz)
 
-let parse32_bounded_integer_le_2
-= [@inline_let] let _ =
-    bounded_integer_of_le_injective 2
-  in
-  make_total_constant_size_parser32
-    2
-    2ul
-    (bounded_integer_of_le 2)
-    ()
-    bounded_integer_of_le_32_2
-
-let parse32_bounded_integer_le_3
-= [@inline_let] let _ =
-    bounded_integer_of_le_injective 3
-  in
-  make_total_constant_size_parser32
-    3
-    3ul
-    (bounded_integer_of_le 3)
-    ()
-    bounded_integer_of_le_32_3
-
-let parse32_bounded_integer_le_4
-= [@inline_let] let _ =
-    bounded_integer_of_le_injective 4
-  in
-  make_total_constant_size_parser32
-    4
-    4ul
-    (bounded_integer_of_le 4)
-    ()
-    bounded_integer_of_le_32_4
-
+let parse32_bounded_integer_le_1 = parse32_bounded_integer_le' 1
+let parse32_bounded_integer_le_2 = parse32_bounded_integer_le' 2
+let parse32_bounded_integer_le_3 = parse32_bounded_integer_le' 3
+let parse32_bounded_integer_le_4 = parse32_bounded_integer_le' 4
 
 let parse32_u16_le =
   parse32_synth'
@@ -198,60 +199,33 @@ let parse32_u32_le =
     parse32_bounded_integer_le_4
     ()
 
-let serialize32_bounded_integer_le_1 = fun (x: bounded_integer 1) -> ((
-    [@inline_let] let _ =
-      serialize_bounded_integer_le_1_eq x 0
-    in
-    B32.create 1ul (Cast.uint32_to_uint8 x)
-  ) <: (res: bytes32 { serializer32_correct' (serialize_bounded_integer_le 1) x res } ))
+inline_for_extraction
+noextract
+let n_to_le_1 = norm [delta_attr [`%E.must_reduce]; iota; zeta; primops] (E.mk_n_to_le (EI.bounded_integer 1) 1)
 
-let serialize32_bounded_integer_le_2
-= fun (x: bounded_integer 2) -> ((
-    [@inline_let] let _ =
-      serialize_bounded_integer_le_2_eq x 0;
-      serialize_bounded_integer_le_2_eq x 1
-    in
-    B32.create 1ul (Cast.uint32_to_uint8 x) `B32.append` B32.create 1ul (Cast.uint32_to_uint8 (x `U32.div` 256ul))
-  ) <: (res: bytes32 { serializer32_correct' (serialize_bounded_integer_le 2) x res } ))
+let serialize32_bounded_integer_le_1 = fun (x: bounded_integer 1) ->
+  n_to_le_1 x
 
-let serialize32_bounded_integer_le_3
-= fun (x: bounded_integer 3) -> ((
-    [@inline_let] let _ =
-      serialize_bounded_integer_le_3_eq x 0;
-      serialize_bounded_integer_le_3_eq x 1;
-      serialize_bounded_integer_le_3_eq x 2
-    in
-    let rem0 = Cast.uint32_to_uint8 x in
-    let div0 = x `U32.div` 256ul in
-    let rem1 = Cast.uint32_to_uint8 div0 in
-    let div1 = div0 `U32.div` 256ul in
-    let rem2 = Cast.uint32_to_uint8 div1 in
-    (B32.create 1ul rem0 `B32.append` B32.create 1ul rem1) `B32.append`
-    B32.create 1ul rem2
-  ) <: (res: bytes32 { serializer32_correct' (serialize_bounded_integer_le 3) x res } ))
+inline_for_extraction
+noextract
+let n_to_le_2 = norm [delta_attr [`%E.must_reduce]; iota; zeta; primops] (E.mk_n_to_le (EI.bounded_integer 2) 2)
 
-#push-options "--z3rlimit 16"
+let serialize32_bounded_integer_le_2 = fun (x: bounded_integer 2) ->
+  n_to_le_2 x
 
-let serialize32_bounded_integer_le_4
-= fun (x: bounded_integer 4) -> ((
-    [@inline_let] let _ =
-      serialize_bounded_integer_le_4_eq x 0;
-      serialize_bounded_integer_le_4_eq x 1;
-      serialize_bounded_integer_le_4_eq x 2;
-      serialize_bounded_integer_le_4_eq x 3
-    in
-    let rem0 = Cast.uint32_to_uint8 x in
-    let div0 = x `U32.div` 256ul in
-    let rem1 = Cast.uint32_to_uint8 div0 in
-    let div1 = div0 `U32.div` 256ul in
-    let rem2 = Cast.uint32_to_uint8 div1 in
-    let div2 = div1 `U32.div` 256ul in
-    let rem3 = Cast.uint32_to_uint8 div2 in
-    (B32.create 1ul rem0 `B32.append` B32.create 1ul rem1) `B32.append`
-    (B32.create 1ul rem2 `B32.append` B32.create 1ul rem3)
-  ) <: (res: bytes32 { serializer32_correct' (serialize_bounded_integer_le 4) x res } ))
+inline_for_extraction
+noextract
+let n_to_le_3 = norm [delta_attr [`%E.must_reduce]; iota; zeta; primops] (E.mk_n_to_le (EI.bounded_integer 3) 3)
 
-#pop-options
+let serialize32_bounded_integer_le_3 = fun (x: bounded_integer 3) ->
+  n_to_le_3 x
+
+inline_for_extraction
+noextract
+let n_to_le_4 = norm [delta_attr [`%E.must_reduce]; iota; zeta; primops] (E.mk_n_to_le (EI.bounded_integer 4) 4)
+
+let serialize32_bounded_integer_le_4 = fun (x: bounded_integer 4) ->
+  n_to_le_4 x
 
 let serialize32_u16_le =
   serialize32_synth' 
