src/lowparse/LowParse.Spec.Endianness.Instances.fst
@@ -1,0 +1,79 @@
+module LowParse.Spec.Endianness.Instances
+include LowParse.Spec.Endianness
+
+module U8 = FStar.UInt8
+
+inline_for_extraction
+noextract
+let uint8 : uinttype U8.t 1 =
+  UIntType
+    (fun x -> U8.v x)
+    (fun x -> x)
+    (fun x -> x)
+    0uy
+    (fun _ _ -> ())
+    (fun x y -> x `U8.add` y)
+    (fun x -> 0uy)
+    (fun x -> 0uy)
+
+module U16 = FStar.UInt16
+
+inline_for_extraction
+noextract
+let uint16 : uinttype U16.t 2 =
+  UIntType
+    (fun x -> U16.v x)
+    (fun x -> FStar.Int.Cast.uint16_to_uint8 x)
+    (fun x -> FStar.Int.Cast.uint8_to_uint16 x)
+    0us
+    (fun _ _ -> ())
+    (fun x y -> x `U16.add` y)
+    (fun x -> x `U16.mul` 256us)
+    (fun x -> x `U16.div` 256us)
+
+module U32 = FStar.UInt32
+
+inline_for_extraction
+noextract
+let uint32 : uinttype U32.t 4 =
+  UIntType
+    (fun x -> U32.v x)
+    (fun x -> FStar.Int.Cast.uint32_to_uint8 x)
+    (fun x -> FStar.Int.Cast.uint8_to_uint32 x)
+    0ul
+    (fun _ _ -> ())
+    (fun x y -> x `U32.add` y)
+    (fun x -> x `U32.mul` 256ul)
+    (fun x -> x `U32.div` 256ul)
+
+module U64 = FStar.UInt64
+
+inline_for_extraction
+noextract
+let uint64 : uinttype U64.t 8 =
+  UIntType
+    (fun x -> U64.v x)
+    (fun x -> FStar.Int.Cast.uint64_to_uint8 x)
+    (fun x -> FStar.Int.Cast.uint8_to_uint64 x)
+    0uL
+    (fun _ _ -> ())
+    (fun x y -> x `U64.add` y)
+    (fun x -> x `U64.mul` 256uL)
+    (fun x -> x `U64.div` 256uL)
+
+open LowParse.Spec.BoundedInt
+
+inline_for_extraction
+noextract
+let bounded_integer
+  (i: integer_size)
+: Tot (uinttype (bounded_integer i) i)
+= UIntType
+    (fun (x: bounded_integer i) -> bounded_integer_prop_equiv i x; U32.v x)
+    (fun x -> FStar.Int.Cast.uint32_to_uint8 x)
+    (fun x -> FStar.Int.Cast.uint8_to_uint32 x)
+    0ul
+    (fun _ _ -> ())
+    (fun x y -> x `U32.add` y)
+    (fun x -> x `U32.mul` 256ul)
+    (fun x -> x `U32.div` 256ul)
