src/lowparse/LowParse.Spec.Endianness.fst
@@ -1,0 +1,22 @@
+module LowParse.Spec.Endianness
+include LowParse.Endianness
+
+module U8 = FStar.UInt8
+module E = LowParse.Endianness
+
+open FStar.Mul
+
+inline_for_extraction
+noextract
+noeq
+type uinttype (t: Type0) (n: nat) =
+  | UIntType:
+    (v: (t -> Tot (y: nat { y < pow2 (8 * n) } ))) ->
+    (to_byte: ((x: t) -> Tot (y: U8.t { U8.v y == v x % 256 } ))) ->
+    (from_byte: ((x: U8.t) -> Tot (y: t { v y == U8.v x } ))) ->
+    (zero: t { v zero == 0 } ) ->
+    (v_inj: ((x1: t) -> (x2: t) -> Lemma (requires (v x1 == v x2)) (ensures (x1 == x2)))) ->
+    (add: ((x: t) -> (y: t) -> Pure t (requires (v x + v y < pow2 (8 * n))) (ensures (fun z -> v z == v x + v y)))) ->
+    (mul256: ((x: t) -> Pure t (requires (v x * 256 < pow2 (8 * n))) (ensures (fun z -> v z == v x * 256)))) ->
+    (div256: ((x: t) -> Pure t (requires True) (ensures (fun z -> v z == v x / 256)))) ->
+    uinttype t n
